Morris86.v basically complete. (ordinal number part remained)

Babel/Framework/Isomorphism.v
@@ -1,6 +1,7 @@
 (** Isomorphism.v *)
-(*
+
 From Babel Require Import TerminalDogma.
+From Coq Require Import Relations.
 
 Set Implicit Arguments.
 Unset Strict Implicit.
@@ -10,13 +11,13 @@ Declare Scope Iso_scope.
 Global Open Scope Iso_scope.
 
 (** A and B are isomorphic types, if there exists a bijection between A and B *)
-Definition isomorphic (A B : Type) :=
-    exists f : A -> B, bijective f.
+Definition isomorphic (A B : Type) := bijection A B.
 Notation " A '≅' B " := (isomorphic A B) (at level 25) : Iso_scope.
 
-Lemma isomorphic_refl : Relation_Definitions.reflexive _ isomorphic.
-Proof. rewrite /Relation_Definitions.reflexive => X.
-    exists ssrfun.id. by apply id_bijective. 
+(*
+Lemma isomorphic_refl : reflexive _ isomorphic.
+Proof. rewrite /reflexive => X.
+    exists ssrfun.id. econstructor. by apply id_bijective. 
 Qed.
 
 Lemma isomorphic_symm : Relation_Definitions.symmetric _ isomorphic.
@@ -29,11 +30,12 @@ Lemma isomorphic_trans : Relation_Definitions.transitive _ isomorphic.
 Proof. rewrite /Relation_Definitions.transitive => X Y Z [f Hf] [g Hg].
     exists (g ◦ f). by apply comp_bijective.
 Qed.
-
+    
 Add Parametric Relation (X Y : Type) : Type isomorphic
     reflexivity proved by isomorphic_refl
     symmetry proved by isomorphic_symm
     transitivity proved by isomorphic_trans as rel_iso.
+*)
 
 Definition IsomorphicExtensionality := forall A B:Type, A ≅ B -> A = B.
 
@@ -49,10 +51,3 @@ Definition IsomorphicExtensionality := forall A B:Type, A ≅ B -> A = B.
 
 Theorem iso_comp (A B C D : Type) : A ≅ B -> C ≅ D -> (A -> C) ≅ (B -> D).
 Abort.
-
-
-Theorem fin_inf_neq : forall n : nat, {x | 1 <= x <= n} <> nat.
-Proof. move => n H. 
-    have Hcontra : {x | 1 <= x <= n} ≅ nat. { rewrite H. apply isomorphic_refl. }
-Admitted.
-*)
