Babel/Framework/Equality.v
@@ -1,0 +1,12 @@
+(** Equality.v *)
+
+From Babel Require Import TerminalDogma.
+
+Set Implicit Arguments.
+Unset Strict Implicit.
+Unset Printing Implicit Defensive.
+
+
+Lemma refl_iff_True (T : Type) (a : T) :
+    a = a <-> True.
+Proof. by []. Qed.
