Babel/LogicFacility/LogicBasic.v
@@ -1,0 +1,19 @@
+(** * LogicBasic.v*)
+
+
+From Babel Require Import TerminalDogma.
+
+Set Implicit Arguments.
+Unset Strict Implicit.
+Unset Printing Implicit Defensive.
+
+Lemma iff_True_R (P : Prop) :
+    (P <-> True) <-> P.
+Proof. split. by move ->. by move => HP; split. Qed.
+
+Lemma iff_True_L (P : Prop) :
+    (True <-> P) <-> P.
+Proof. split. 
+    move => H. symmetry in H. by rewrite iff_True_R in H. 
+    by [].
+Qed.
