Babel/LogicFacility/LogicFacility.v
@@ -1,0 +1,2 @@
+
+From Babel.LogicFacility Require Export LogicBasic.
