experimental/other.v
@@ -1,0 +1,7 @@
+
+(*
+Theorem fin_inf_neq : forall n : nat, {x | 1 <= x <= n} <> nat.
+Proof. move => n H. 
+    have Hcontra : {x | 1 <= x <= n} ≅ nat. { rewrite H. apply isomorphic_refl. }
+Admitted.
+*)
